SystemFD/Term/VariableSet.lean
@@ -1,6 +1,7 @@
 import SystemFD.Substitution
 import SystemFD.Ctx
 import SystemFD.Term.Definition
+import SystemFD.Term.Substitution
 
 namespace List
   @[simp]
@@ -8,15 +9,42 @@ namespace List
 end List
 
 namespace Term
+
   @[simp]
-  def vars : Term -> List Nat
-  | var x => [x]
+  def vars_inner (c : Nat) : Term -> List Nat
+  | var x => if c.ble x then [x - c] else []
   | kind => []
   | type => []
-  | ctor1 _ t => vars t
-  | ctor2 _ t1 t2 => vars t1 ++ vars t2
-  | bind2 _ t1 t2 => vars t1 ++ vars t2
-  | ite t1 t2 t3 t4 => vars t1 ++ vars t2 ++ vars t3 ++ vars t4
-  | guard t1 t2 t3 => vars t1 ++ vars t2 ++ vars t3
-  | letterm t1 t2 t3 => vars t1 ++ vars t2 ++ vars t3
+  | ctor1 _ t => vars_inner c t
+  | ctor2 _ t1 t2 => vars_inner c t1 ++ vars_inner c t2
+  | bind2 _ t1 t2 => vars_inner c t1 ++ vars_inner (c + 1) t2
+  | ite t1 t2 t3 t4 => vars_inner c t1 ++ vars_inner c t2 ++ vars_inner c t3 ++ vars_inner c t4
+  | guard t1 t2 t3 => vars_inner c t1 ++ vars_inner c t2 ++ vars_inner c t3
+  | letterm t1 t2 t3 => vars_inner c t1 ++ vars_inner c t2 ++ vars_inner (c + 1) t3
+
+  def vars (t : Term) : List Nat := vars_inner 0 t
+
+  -- theorem zero_not_var_inner (r : Ren) (σ : Subst Term) :
+  --   (∀ x, c ≤ x -> (x - c) ∉ Term.vars_inner c t) ->
+  --   (∀ n, n ≥ c -> σ n = r.to n) ->
+  --   [σ]t = [r.to]t
+  -- := by sorry
+
+  -- theorem zero_not_var_implies_beta_noop {t : Term} a :
+  --   0 ∉ t.vars -> t β[a] = [P]t
+  -- := by
+  -- intro h
+  -- induction t <;> simp at *
+  -- case _ y =>
+  --   unfold Term.vars at h
+  --   cases y <;> simp at *
+  -- case _ ih => apply ih h
+  -- case _ ih1 ih2 => sorry
+  -- case _ ih1 ih2 =>
+
+  --   sorry
+  -- case _ => sorry
+  -- case _ => sorry
+  -- case _ => sorry
+
 end Term
